src/program_proof/tulip/program/backup/bgcoord_send.v
@@ -1,24 +1,298 @@
 From Perennial.program_proof.tulip.program Require Import prelude.
+(* import it for [encode] *)
+From Perennial.program_proof.tulip.program.gcoord Require Import encode.
 From Perennial.program_proof.tulip.program.backup Require Import bgcoord_repr.
 
 Section program.
   Context `{!heapGS Σ, !tulip_ghostG Σ}.
 
+  Theorem wp_BackupGroupCoordinator__GetConnection
+    (gcoord : loc) (rid : u64) (addrm : gmap u64 chan) (addr : chan)
+    rk ts gid γ :
+    addrm !! rid = Some addr ->
+    is_backup_gcoord_with_addrm gcoord addrm rk ts gid γ -∗
+    {{{ True }}}
+      BackupGroupCoordinator__GetConnection #gcoord #rid
+    {{{ (trml : chan) (ok : bool), RET (if ok 
+                                     then (connection_socket trml addr, #true)
+                                     else (#(), #false));
+        if ok then is_terminal γ gid trml else True
+    }}}.
+  Proof.
+    iIntros (Haddr) "#Hgcoord".
+    iIntros (Φ) "!> _ HΦ".
+    wp_rec.
+
+    (*@ func (gcoord *GroupCoordinator) GetConnection(rid uint64) (grove_ffi.Connection, bool) { @*)
+    (*@     gcoord.mu.Lock()                                                    @*)
+    (*@     conn, ok := gcoord.conns[rid]                                       @*)
+    (*@     gcoord.mu.Unlock()                                                  @*)
+    (*@     return conn, ok                                                     @*)
+    (*@ }                                                                       @*)
+    iNamed "Hgcoord".
+    wp_loadField.
+    wp_apply (wp_Mutex__Lock with "Hlock").
+    iIntros "[Hlocked Hgcoord]".
+    iNamed "Hgcoord".
+    iNamed "Hcomm".
+    wp_loadField.
+    wp_apply (map.wp_MapGet with "Hconns").
+    iIntros (connV ok) "[%Hok Hconns]".
+    wp_pures.
+    wp_loadField.
+    wp_apply (wp_Mutex__Unlock with "[-HΦ]").
+    { by iFrame "Hlock Hlocked ∗ # %". }
+    wp_pures.
+    destruct ok; last first.
+    { apply map.map_get_false in Hok as [_ ->].
+      (* [U64 0] is a placeholder *)
+      by iApply ("HΦ" $! (U64 0) false).
+    }
+    apply map.map_get_true in Hok.
+    rewrite lookup_fmap_Some in Hok.
+    destruct Hok as ([trml addr'] & <- & Hconns).
+    iDestruct (big_sepM_lookup with "Htrmls") as "Htrml"; first apply Hconns.
+    apply Haddrm in Hconns.
+    rewrite Haddr in Hconns.
+    symmetry in Hconns. inv Hconns.
+    by iApply ("HΦ" $! _ true).
+  Qed.
+
+  Theorem wp_BackupGroupCoordinator__Connect
+    (gcoord : loc) (rid : u64) (addrm : gmap u64 chan) (addr : chan) rk ts gid γ :
+    addrm !! rid = Some addr ->
+    is_backup_gcoord_with_addrm gcoord addrm rk ts gid γ -∗
+    {{{ True }}}
+      BackupGroupCoordinator__Connect #gcoord #rid
+    {{{ (ok : bool), RET #ok; True }}}.
+  Proof.
+    iIntros (Haddr) "#Hgcoord".
+    iIntros (Φ) "!> _ HΦ".
+    wp_rec.
+
+    (*@ func (gcoord *GroupCoordinator) Connect(rid uint64) bool {              @*)
+    (*@     addr := gcoord.addrm[rid]                                           @*)
+    (*@     ret := grove_ffi.Connect(addr)                                      @*)
+    (*@     if !ret.Err {                                                       @*)
+    (*@         gcoord.mu.Lock()                                                @*)
+    (*@         gcoord.conns[rid] = ret.Connection                              @*)
+    (*@         gcoord.mu.Unlock()                                              @*)
+    (*@         return true                                                     @*)
+    (*@     }                                                                   @*)
+    (*@     return false                                                        @*)
+    (*@ }                                                                       @*)
+    iNamed "Hgcoord". iNamed "Haddrm".
+    wp_loadField.
+    wp_apply (wp_MapGet with "Haddrm").
+    iIntros (addrpeer' ok) "[%Hok _]".
+    destruct ok; last first.
+    { apply map_get_false in Hok as [Hok _].
+      by rewrite Haddr in Hok.
+    }
+    apply map_get_true in Hok.
+    rewrite Haddr in Hok.
+    symmetry in Hok. inv Hok.
+    wp_pures.
+    wp_apply wp_Connect.
+    iIntros (err trml) "Htrml".
+    wp_pures.
+    wp_if_destruct.
+    { wp_loadField.
+      wp_apply (wp_Mutex__Lock with "Hlock").
+      iIntros "[Hlocked Hgcoord]".
+      iNamed "Hgcoord". iNamed "Hcomm".
+      wp_loadField.
+      wp_apply (map.wp_MapInsert with "Hconns").
+      iIntros "Hconns".
+      wp_loadField.
+      (* Seal [trml c↦ ∅] in the network invariant and obtain [is_terminal γ trml]. *)
+      iApply ncfupd_wp.
+      iInv "Hinvnet" as "> HinvnetO" "HinvnetC".
+      iNamed "HinvnetO".
+      iMod (terminal_update trml with "Hterminals") as "[Hterminals #Htrmlrcpt]".
+      iMod ("HinvnetC" with "[$Hlistens Hconnects Hterminals Htrml]") as "_".
+      { iModIntro.
+        iExists (<[trml := ∅]> connects).
+        rewrite dom_insert_L.
+        iFrame "Hterminals %".
+        iApply (big_sepM_insert_2 with "[Htrml] Hconnects").
+        iExists ∅.
+        iFrame.
+        iSplit; first by rewrite big_sepS_empty.
+        done.
+      }
+      iModIntro.
+      wp_apply (wp_Mutex__Unlock with "[$Hlock $Hlocked $HconnsP $Hgpp Hconns]").
+      { iModIntro.
+        iExists (<[rid := (trml, addr)]> conns).
+        rewrite fmap_insert.
+        iFrame "Hconns".
+        iSplit.
+        { by iApply big_sepM_insert_2. }
+        iPureIntro.
+        by apply map_Forall_insert_2.
+      }
+      wp_pures.
+      by iApply "HΦ".
+    }
+    by iApply "HΦ".
+  Qed.
+
+  Theorem wp_BackupGroupCoordinator__Send
+    (gcoord : loc) (rid : u64) (dataP : Slice.t) (data : list u8)
+    (addrm : gmap u64 chan) (addr : chan) rk ts gid γ :
+    addrm !! rid = Some addr ->
+    is_backup_gcoord_with_addrm gcoord addrm rk ts gid γ -∗
+    {{{ own_slice dataP byteT (DfracOwn 1) data }}}
+    <<< ∀∀ ms, addr c↦ ms >>>
+      BackupGroupCoordinator__Send #gcoord #rid (to_val dataP) @ ∅
+    <<< ∃∃ (ok : bool),
+            if ok
+            then ∃ trml, addr c↦ ({[Message trml data]} ∪ ms) ∗ is_terminal γ gid trml
+            else addr c↦ ms
+    >>>
+    {{{ RET #(); True }}}.
+  Proof.
+    iIntros (Haddr) "#Hgcoord".
+    iIntros (Φ) "!> Hdata HAU".
+    wp_rec.
+
+    (*@ func (gcoord *GroupCoordinator) Send(rid uint64, data []byte) {         @*)
+    (*@     conn, ok := gcoord.GetConnection(rid)                               @*)
+    (*@     if !ok {                                                            @*)
+    (*@         gcoord.Connect(rid)                                             @*)
+    (*@         return                                                          @*)
+    (*@     }                                                                   @*)
+    (*@                                                                         @*)
+    wp_apply (wp_BackupGroupCoordinator__GetConnection with "Hgcoord").
+    { apply Haddr. }
+    iIntros (trml ok) "#Htrmlrcpt".
+    wp_pures.
+    destruct ok; wp_pures; last first.
+    { wp_apply (wp_BackupGroupCoordinator__Connect with "Hgcoord").
+      { apply Haddr. }
+      iIntros (ok) "Hok".
+      wp_pures.
+      (* Open the AU without updating. *)
+      iMod (ncfupd_mask_subseteq (⊤ ∖ ∅)) as "Hclose"; first solve_ndisj.
+      iMod "HAU" as (ms) "[Hms HAU]".
+      iMod ("HAU" $! false with "Hms") as "HΦ".
+      iMod "Hclose" as "_".
+      by iApply "HΦ".
+    }
+
+    (*@     err := grove_ffi.Send(conn, data)                                   @*)
+    (*@     if err {                                                            @*)
+    (*@         gcoord.Connect(rid)                                             @*)
+    (*@     }                                                                   @*)
+    (*@ }                                                                       @*)
+    iDestruct (own_slice_to_small with "Hdata") as "Hdata".
+    wp_apply (wp_Send with "Hdata").
+    iMod "HAU" as (ms) "[Hms HAU]".
+    iFrame "Hms".
+    iIntros "!>" (sent) "Hms".
+    iMod ("HAU" $! sent with "[Hms]") as "HΦ".
+    { rewrite union_comm_L. by destruct sent; first iFrame. }
+    iModIntro.
+    iIntros (err) "[%Herr Hdata]".
+    wp_pures.
+    wp_if_destruct.
+    { wp_apply (wp_BackupGroupCoordinator__Connect with "Hgcoord").
+      { apply Haddr. }
+      iIntros (ok) "_".
+      wp_pures.
+      by iApply "HΦ".
+    }
+    by iApply "HΦ".
+  Qed.
+
   Theorem wp_BackupGroupCoordinator__SendInquire
     (gcoord : loc) (rid : u64) (tsW : u64) (rankW : u64) (cid : coordid) addrm gid γ :
     let ts := uint.nat tsW in
     let rank := uint.nat rankW in
+    valid_ts ts ->
     rid ∈ dom addrm ->
     is_backup_gcoord_with_addrm gcoord addrm rank ts gid γ -∗
     {{{ True }}}
       BackupGroupCoordinator__SendInquire #gcoord #rid #tsW #rankW (coordid_to_val cid)
     {{{ RET #(); True }}}.
   Proof.
+    iIntros (ts rank Hvts Hrid) "#Hgcoord".
+    iIntros (Φ) "!> Hpwrs HΦ".
+    wp_rec.
+
     (*@ func (gcoord *BackupGroupCoordinator) SendInquire(rid, ts, rank uint64) { @*)
     (*@     data := message.EncodeTxnInquireRequest(ts, rank)                   @*)
     (*@     gcoord.Send(rid, data)                                              @*)
     (*@ }                                                                       @*)
-  Admitted.
+    wp_apply (wp_EncodeTxnInquireRequest).
+    iIntros (dataP data) "(Hdata & %Hdataenc)".
+    iNamed "Hgcoord".
+    iNamed "Haddrm".
+    assert (is_Some (addrm !! rid)) as [addrpeer Haddrpeer].
+    { by apply elem_of_dom. }
+    wp_apply (wp_BackupGroupCoordinator__Send with "[] Hdata"); first apply Haddrpeer.
+    { by iFrame "HcvP # %". }
+    iInv "Hinvnet" as "> HinvnetO" "HinvnetC".
+    iApply ncfupd_mask_intro; first set_solver.
+    iIntros "Hmask".
+    iNamed "HinvnetO".
+    assert (is_Some (listens !! addrpeer)) as [ms Hms].
+    { rewrite -elem_of_dom -Himgaddrm elem_of_map_img. by eauto. }
+    iDestruct (big_sepM_delete with "Hlistens") as "[Hlst Hlistens]"; first apply Hms.
+    iNamed "Hlst".
+    iFrame "Hms".
+    iIntros (sent) "Hms".
+    destruct sent; last first.
+    { iDestruct (big_sepM_insert_2 _ _ addrpeer ms with "[Hms] Hlistens") as "Hlistens".
+      { iFrame "∗ # %". }
+      rewrite insert_delete; last apply Hms.
+      iMod "Hmask" as "_".
+      iMod ("HinvnetC" with "[$Hlistens $Hconnects $Hterminals]") as "_".
+      { done. }
+      iIntros "!> _".
+      wp_pures.
+      by iApply "HΦ".
+    }
+    iDestruct "Hms" as (trml) "[Hms #Htrml]".
+    set ms' := _ ∪ ms.
+    iDestruct (big_sepM_insert_2 _ _ addrpeer ms' with "[Hms] Hlistens") as "Hlistens".
+    { iFrame "Hms".
+      set req := InquireReq _ _ _ in Hdataenc.
+      iExists ({[req]} ∪ reqs).
+      iSplit.
+      { rewrite set_map_union_L set_map_singleton_L.
+        by iApply big_sepS_insert_2.
+      }
+      iSplit.
+      { iApply big_sepS_insert_2; last done.
+        simpl.
+        iPureIntro.
+        split; first apply Hvts.
+        rewrite /valid_backup_rank.
+        clear -Hrk. word.
+      }
+      (* { iApply big_sepS_insert_2; [admit | done]. } *)
+      iPureIntro.
+      apply set_Forall_union; last first.
+      { apply (set_Forall_impl _ _ _ Henc). intros m Hm. clear -Hm. set_solver. }
+      rewrite set_Forall_singleton.
+      exists req.
+      split; first set_solver.
+      done.
+    }
+    rewrite insert_delete_insert.
+    iMod "Hmask" as "_".
+    iMod ("HinvnetC" with "[$Hlistens $Hconnects $Hterminals]") as "_".
+    { iPureIntro.
+      rewrite dom_insert_L Himgaddrm.
+      apply (elem_of_map_img_2 (SA := gset chan)) in Haddrpeer.
+      set_solver.
+    }
+    iIntros "!> _".
+    wp_pures.
+    by iApply "HΦ".
+  Qed.
 
   Theorem wp_BackupGroupCoordinator__SendValidate
     (gcoord : loc) (rid : u64) (tsW : u64) (rankW : u64) (pwrsP : loc) (ptgsP : Slice.t)
@@ -33,11 +307,75 @@ Section program.
       BackupGroupCoordinator__SendValidate #gcoord #rid #tsW #rankW #pwrsP (to_val ptgsP)
     {{{ RET #(); True }}}.
   Proof.
+    iIntros (ts rank Hrid) "#Hsafepwrs #Hptgs #Hgcoord".
+    iIntros (Φ) "!> Hpwrs HΦ".
+    wp_rec.
+
     (*@ func (gcoord *BackupGroupCoordinator) SendValidate(rid, ts, rank uint64, pwrs tulip.KVMap, ptgs []uint64) { @*)
     (*@     data := message.EncodeTxnValidateRequest(ts, rank, pwrs, ptgs)      @*)
     (*@     gcoord.Send(rid, data)                                              @*)
     (*@ }                                                                       @*)
-  Admitted.
+    wp_apply (wp_EncodeTxnValidateRequest with "Hptgs Hpwrs").
+    iIntros (dataP data) "(Hdata & Hpwrs & %Hdataenc)".
+    iNamed "Hgcoord".
+    iNamed "Haddrm".
+    assert (is_Some (addrm !! rid)) as [addrpeer Haddrpeer].
+    { by apply elem_of_dom. }
+    wp_apply (wp_BackupGroupCoordinator__Send with "[] Hdata"); first apply Haddrpeer.
+    { by iFrame "HcvP # %". }
+    iInv "Hinvnet" as "> HinvnetO" "HinvnetC".
+    iApply ncfupd_mask_intro; first set_solver.
+    iIntros "Hmask".
+    iNamed "HinvnetO".
+    assert (is_Some (listens !! addrpeer)) as [ms Hms].
+    { rewrite -elem_of_dom -Himgaddrm elem_of_map_img. by eauto. }
+    iDestruct (big_sepM_delete with "Hlistens") as "[Hlst Hlistens]"; first apply Hms.
+    iNamed "Hlst".
+    iFrame "Hms".
+    iIntros (sent) "Hms".
+    destruct sent; last first.
+    { iDestruct (big_sepM_insert_2 _ _ addrpeer ms with "[Hms] Hlistens") as "Hlistens".
+      { iFrame "∗ # %". }
+      rewrite insert_delete; last apply Hms.
+      iMod "Hmask" as "_".
+      iMod ("HinvnetC" with "[$Hlistens $Hconnects $Hterminals]") as "_".
+      { done. }
+      iIntros "!> _".
+      wp_pures.
+      by iApply "HΦ".
+    }
+    iDestruct "Hms" as (trml) "[Hms #Htrml]".
+    set ms' := _ ∪ ms.
+    iDestruct (big_sepM_insert_2 _ _ addrpeer ms' with "[Hms] Hlistens") as "Hlistens".
+    { iFrame "Hms".
+      set req := ValidateReq _ _ _ _ in Hdataenc.
+      iExists ({[req]} ∪ reqs).
+      iSplit.
+      { rewrite set_map_union_L set_map_singleton_L.
+        by iApply big_sepS_insert_2.
+      }
+      iSplit.
+      { iApply big_sepS_insert_2; [done | done]. }
+      iPureIntro.
+      apply set_Forall_union; last first.
+      { apply (set_Forall_impl _ _ _ Henc). intros m Hm. clear -Hm. set_solver. }
+      rewrite set_Forall_singleton.
+      exists req.
+      split; first set_solver.
+      done.
+    }
+    rewrite insert_delete_insert.
+    iMod "Hmask" as "_".
+    iMod ("HinvnetC" with "[$Hlistens $Hconnects $Hterminals]") as "_".
+    { iPureIntro.
+      rewrite dom_insert_L Himgaddrm.
+      apply (elem_of_map_img_2 (SA := gset chan)) in Haddrpeer.
+      set_solver.
+    }
+    iIntros "!> _".
+    wp_pures.
+    by iApply "HΦ".
+  Qed.
 
   Theorem wp_BackupGroupCoordinator__SendPrepare
     (gcoord : loc) (rid : u64) (tsW : u64) (rankW : u64) addrm gid γ :
@@ -50,11 +388,75 @@ Section program.
       BackupGroupCoordinator__SendPrepare #gcoord #rid #tsW #rankW
     {{{ RET #(); True }}}.
   Proof.
+    iIntros (ts rank Hrid) "#Hppsl #Hgcoord".
+    iIntros (Φ) "!> _ HΦ".
+    wp_rec.
+
     (*@ func (gcoord *BackupGroupCoordinator) SendPrepare(rid, ts, rank uint64) { @*)
     (*@     data := message.EncodeTxnPrepareRequest(ts, rank)                   @*)
     (*@     gcoord.Send(rid, data)                                              @*)
     (*@ }                                                                       @*)
-  Admitted.
+    wp_apply (wp_EncodeTxnPrepareRequest).
+    iIntros (dataP data) "(Hdata & %Hdataenc)".
+    iNamed "Hgcoord".
+    iNamed "Haddrm".
+    assert (is_Some (addrm !! rid)) as [addrpeer Haddrpeer].
+    { by apply elem_of_dom. }
+    wp_apply (wp_BackupGroupCoordinator__Send with "[] Hdata"); first apply Haddrpeer.
+    { by iFrame "HcvP # %". }
+    iInv "Hinvnet" as "> HinvnetO" "HinvnetC".
+    iApply ncfupd_mask_intro; first set_solver.
+    iIntros "Hmask".
+    iNamed "HinvnetO".
+    assert (is_Some (listens !! addrpeer)) as [ms Hms].
+    { rewrite -elem_of_dom -Himgaddrm elem_of_map_img. by eauto. }
+    iDestruct (big_sepM_delete with "Hlistens") as "[Hlst Hlistens]"; first apply Hms.
+    iNamed "Hlst".
+    iFrame "Hms".
+    iIntros (sent) "Hms".
+    destruct sent; last first.
+    { iDestruct (big_sepM_insert_2 _ _ addrpeer ms with "[Hms] Hlistens") as "Hlistens".
+      { iFrame "∗ # %". }
+      rewrite insert_delete; last apply Hms.
+      iMod "Hmask" as "_".
+      iMod ("HinvnetC" with "[$Hlistens $Hconnects $Hterminals]") as "_".
+      { done. }
+      iIntros "!> _".
+      wp_pures.
+      by iApply "HΦ".
+    }
+    iDestruct "Hms" as (trml) "[Hms #Htrml]".
+    set ms' := _ ∪ ms.
+    iDestruct (big_sepM_insert_2 _ _ addrpeer ms' with "[Hms] Hlistens") as "Hlistens".
+    { iFrame "Hms".
+      set req := PrepareReq _ _ in Hdataenc.
+      iExists ({[req]} ∪ reqs).
+      iSplit.
+      { rewrite set_map_union_L set_map_singleton_L.
+        by iApply big_sepS_insert_2.
+      }
+      iSplit.
+      { iApply big_sepS_insert_2; last done. iFrame "Hppsl". iPureIntro. clear -Hrk. word. }
+      iPureIntro.
+      apply set_Forall_union; last first.
+      { apply (set_Forall_impl _ _ _ Henc). intros m Hm. clear -Hm. set_solver. }
+      rewrite set_Forall_singleton.
+      exists req.
+      split; first set_solver.
+      done.
+    }
+    rewrite insert_delete_insert.
+    iMod "Hmask" as "_".
+    iMod ("HinvnetC" with "[$Hlistens $Hconnects $Hterminals]") as "_".
+    { iPureIntro.
+      rewrite dom_insert_L Himgaddrm.
+      apply (elem_of_map_img_2 (SA := gset chan)) in Haddrpeer.
+      set_solver.
+    }
+    iIntros "!> _".
+    wp_pures.
+    by iApply "HΦ".
+  Qed.
 
   Theorem wp_BackupGroupCoordinator__SendUnprepare
     (gcoord : loc) (rid : u64) (tsW : u64) (rankW : u64) addrm gid γ :
@@ -67,11 +469,75 @@ Section program.
       BackupGroupCoordinator__SendUnprepare #gcoord #rid #tsW #rankW
     {{{ RET #(); True }}}.
   Proof.
+    iIntros (ts rank Hrid) "#Hppsl #Hgcoord".
+    iIntros (Φ) "!> _ HΦ".
+    wp_rec.
+
     (*@ func (gcoord *BackupGroupCoordinator) SendUnprepare(rid, ts, rank uint64) { @*)
     (*@     data := message.EncodeTxnUnprepareRequest(ts, rank)                 @*)
     (*@     gcoord.Send(rid, data)                                              @*)
     (*@ }                                                                       @*)
-  Admitted.
+wp_apply (wp_EncodeTxnUnprepareRequest).
+    iIntros (dataP data) "(Hdata & %Hdataenc)".
+    iNamed "Hgcoord".
+    iNamed "Haddrm".
+    assert (is_Some (addrm !! rid)) as [addrpeer Haddrpeer].
+    { by apply elem_of_dom. }
+    wp_apply (wp_BackupGroupCoordinator__Send with "[] Hdata"); first apply Haddrpeer.
+    { by iFrame "HcvP # %". }
+    iInv "Hinvnet" as "> HinvnetO" "HinvnetC".
+    iApply ncfupd_mask_intro; first set_solver.
+    iIntros "Hmask".
+    iNamed "HinvnetO".
+    assert (is_Some (listens !! addrpeer)) as [ms Hms].
+    { rewrite -elem_of_dom -Himgaddrm elem_of_map_img. by eauto. }
+    iDestruct (big_sepM_delete with "Hlistens") as "[Hlst Hlistens]"; first apply Hms.
+    iNamed "Hlst".
+    iFrame "Hms".
+    iIntros (sent) "Hms".
+    destruct sent; last first.
+    { iDestruct (big_sepM_insert_2 _ _ addrpeer ms with "[Hms] Hlistens") as "Hlistens".
+      { iFrame "∗ # %". }
+      rewrite insert_delete; last apply Hms.
+      iMod "Hmask" as "_".
+      iMod ("HinvnetC" with "[$Hlistens $Hconnects $Hterminals]") as "_".
+      { done. }
+      iIntros "!> _".
+      wp_pures.
+      by iApply "HΦ".
+    }
+    iDestruct "Hms" as (trml) "[Hms #Htrml]".
+    set ms' := _ ∪ ms.
+    iDestruct (big_sepM_insert_2 _ _ addrpeer ms' with "[Hms] Hlistens") as "Hlistens".
+    { iFrame "Hms".
+      set req := UnprepareReq _ _ in Hdataenc.
+      iExists ({[req]} ∪ reqs).
+      iSplit.
+      { rewrite set_map_union_L set_map_singleton_L.
+        by iApply big_sepS_insert_2.
+      }
+      iSplit.
+      { iApply big_sepS_insert_2; last done. iFrame "Hppsl". iPureIntro. clear -Hrk. word. }
+      iPureIntro.
+      apply set_Forall_union; last first.
+      { apply (set_Forall_impl _ _ _ Henc). intros m Hm. clear -Hm. set_solver. }
+      rewrite set_Forall_singleton.
+      exists req.
+      split; first set_solver.
+      done.
+    }
+    rewrite insert_delete_insert.
+    iMod "Hmask" as "_".
+    iMod ("HinvnetC" with "[$Hlistens $Hconnects $Hterminals]") as "_".
+    { iPureIntro.
+      rewrite dom_insert_L Himgaddrm.
+      apply (elem_of_map_img_2 (SA := gset chan)) in Haddrpeer.
+      set_solver.
+    }
+    iIntros "!> _".
+    wp_pures.
+    by iApply "HΦ".
+  Qed.
 
   Theorem wp_BackupGroupCoordinator__SendRefresh
     (gcoord : loc) (rid : u64) (tsW : u64) (rankW : u64) addrm gid γ :
@@ -83,10 +549,74 @@ Section program.
       BackupGroupCoordinator__SendRefresh #gcoord #rid #tsW #rankW
     {{{ RET #(); True }}}.
   Proof.
+    iIntros (ts rank Hrid) "#Hgcoord".
+    iIntros (Φ) "!> _ HΦ".
+    wp_rec.
+
     (*@ func (gcoord *BackupGroupCoordinator) SendRefresh(rid, ts, rank uint64) { @*)
     (*@     data := message.EncodeTxnRefreshRequest(ts, rank)                   @*)
     (*@     gcoord.Send(rid, data)                                              @*)
     (*@ }                                                                       @*)
-  Admitted.
+    wp_apply (wp_EncodeTxnRefreshRequest).
+    iIntros (dataP data) "(Hdata & %Hdataenc)".
+    iNamed "Hgcoord".
+    iNamed "Haddrm".
+    assert (is_Some (addrm !! rid)) as [addrpeer Haddrpeer].
+    { by apply elem_of_dom. }
+    wp_apply (wp_BackupGroupCoordinator__Send with "[] Hdata"); first apply Haddrpeer.
+    { by iFrame "HcvP # %". }
+    iInv "Hinvnet" as "> HinvnetO" "HinvnetC".
+    iApply ncfupd_mask_intro; first set_solver.
+    iIntros "Hmask".
+    iNamed "HinvnetO".
+    assert (is_Some (listens !! addrpeer)) as [ms Hms].
+    { rewrite -elem_of_dom -Himgaddrm elem_of_map_img. by eauto. }
+    iDestruct (big_sepM_delete with "Hlistens") as "[Hlst Hlistens]"; first apply Hms.
+    iNamed "Hlst".
+    iFrame "Hms".
+    iIntros (sent) "Hms".
+    destruct sent; last first.
+    { iDestruct (big_sepM_insert_2 _ _ addrpeer ms with "[Hms] Hlistens") as "Hlistens".
+      { iFrame "∗ # %". }
+      rewrite insert_delete; last apply Hms.
+      iMod "Hmask" as "_".
+      iMod ("HinvnetC" with "[$Hlistens $Hconnects $Hterminals]") as "_".
+      { done. }
+      iIntros "!> _".
+      wp_pures.
+      by iApply "HΦ".
+    }
+    iDestruct "Hms" as (trml) "[Hms #Htrml]".
+    set ms' := _ ∪ ms.
+    iDestruct (big_sepM_insert_2 _ _ addrpeer ms' with "[Hms] Hlistens") as "Hlistens".
+    { iFrame "Hms".
+      set req := RefreshReq _ _ in Hdataenc.
+      iExists ({[req]} ∪ reqs).
+      iSplit.
+      { rewrite set_map_union_L set_map_singleton_L.
+        by iApply big_sepS_insert_2.
+      }
+      iSplit.
+      { by iApply big_sepS_insert_2. }
+      iPureIntro.
+      apply set_Forall_union; last first.
+      { apply (set_Forall_impl _ _ _ Henc). intros m Hm. clear -Hm. set_solver. }
+      rewrite set_Forall_singleton.
+      exists req.
+      split; first set_solver.
+      done.
+    }
+    rewrite insert_delete_insert.
+    iMod "Hmask" as "_".
+    iMod ("HinvnetC" with "[$Hlistens $Hconnects $Hterminals]") as "_".
+    { iPureIntro.
+      rewrite dom_insert_L Himgaddrm.
+      apply (elem_of_map_img_2 (SA := gset chan)) in Haddrpeer.
+      set_solver.
+    }
+    iIntros "!> _".
+    wp_pures.
+    by iApply "HΦ".
+  Qed.
 
 End program.
